Tests/STLC/Fixture.lean
@@ -6,10 +6,10 @@ open Lp2lc.Active.Util
 open Lp2lc.Active.STLC
 
 class TestEnv where
-  trm2val : UIdView (λ T => AST.Val { C := T, D := String })
-  trm2valCtx : UIdEquiv.Extendable.{3, 3}
-    (VK := λ T => AST.Val { C := T, D := String }) (base := trm2val)
-  decidableEq (C : UIdU) : DecidableEq C
+  trm2val : UIdView (λ T => ∀ {B : UIdU}, AST.Val { F := T, B := B, D := String })
+  trm2valExeCtx : UIdEquiv.Extendable.{3, 3}
+    (VK := λ T => AST.Val { F := T, B := trm2val.UId, D := String })
+    (base := { UId := trm2val.UId, get := λ uid => trm2val.get uid (B := trm2val.UId) })
 
 variable [testEnv : TestEnv]
 
